feat: define the problem

KripkeGameAnalysis/Basic.lean
@@ -1,1 +1,129 @@
-def hello := "world"
+import Mathlib.Data.Finset.Basic
+import Mathlib.Data.Finset.Defs
+import Mathlib.Data.Finset.Dedup
+import Mathlib.Data.Finset.Prod
+import Mathlib.Data.Finset.Powerset
+import Mathlib.Data.Fintype.Basic
+import Mathlib.Data.Fintype.Card
+
+import KripkeGameAnalysis.GenericExtras.FinsetEquivCharacteristic
+
+inductive KripkeGameVars : Type
+| p
+| q
+| r
+| s
+deriving Ord, BEq, DecidableEq
+
+instance KripkeGameVars.fintype : Fintype KripkeGameVars :=
+  open KripkeGameVars in
+  ⟨⟨{p, q, r, s}, by simp⟩, fun x => by cases x <;> simp⟩
+
+def KripkeGameVars.all : Finset KripkeGameVars := Finset.univ
+
+inductive ModalFormula : Type
+| var : KripkeGameVars → ModalFormula
+| neg : ModalFormula → ModalFormula
+| and : ModalFormula → ModalFormula → ModalFormula
+| box : ModalFormula → ModalFormula
+
+namespace ModalFormula
+  abbrev p := ModalFormula.var KripkeGameVars.p
+  abbrev q := ModalFormula.var KripkeGameVars.q
+  abbrev r := ModalFormula.var KripkeGameVars.r
+  abbrev s := ModalFormula.var KripkeGameVars.s
+  abbrev not := ModalFormula.neg
+  abbrev or φ1 φ2 := ModalFormula.not (ModalFormula.and (ModalFormula.not φ1) (ModalFormula.not φ2))
+  abbrev implies φ1 φ2 := ModalFormula.or (ModalFormula.not φ1) φ2
+  abbrev dia φ := ModalFormula.not (ModalFormula.box (ModalFormula.not φ))
+end ModalFormula
+
+/-- A Kripke frame of `frameSize` possible worlds is a directed graph with `frameSize` nodes.
+
+We think of the nodes in the graph as being numbered from `0` to `frameSize - 1`, inclusive,
+and we think the `j`-th node is accessible from the `i`-th node if and only if there is an edge from `i` to `j`.
+
+The graph, then, is represented by a function that takes two natural numbers `n` and `m` as input,
+and returns `true` if there is an edge from node `n` to node `m`, and `false` otherwise.
+-/
+def KripkeFrame (frameSize : Nat) : Type := Fin frameSize → Fin frameSize → Bool
+namespace KripkeFrame
+  def Node (_ : KripkeFrame frameSize) := Fin frameSize
+  instance (frame : KripkeFrame n) : Fintype frame.Node := inferInstanceAs (Fintype (Fin n))
+  instance (frame : KripkeFrame n) : DecidableEq frame.Node := inferInstanceAs (DecidableEq (Fin n))
+
+  def allNodes (frame : KripkeFrame n) : Finset frame.Node := Finset.univ
+  lemma allNodes_card_eq_frameSize (frame : KripkeFrame n) : frame.allNodes.card = n :=
+    by apply Fintype.card_fin
+
+  def accessible (frame : KripkeFrame n) (i j : frame.Node) : Bool := frame i j
+  def accessibilityRelationCount (frame : KripkeFrame n) : ℕ :=
+    ((frame.allNodes.product (frame.allNodes)).filter (fun a => frame.accessible a.fst a.snd)).card
+
+  def Valuation (frame : KripkeFrame n) : Type := KripkeGameVars → frame.Node → Bool
+
+  def Valuation.satisfiesAt {frame : KripkeFrame n} (i : frame.Node) (fml : ModalFormula) (val : frame.Valuation) : Bool :=
+  match fml with
+    | ModalFormula.var x => val x i
+    | ModalFormula.neg φ => !(val.satisfiesAt i φ)
+    | ModalFormula.and φ1 φ2 => val.satisfiesAt i φ1 && val.satisfiesAt i φ2
+    | ModalFormula.box φ => decide (∀j ∈ frame.allNodes, if frame.accessible i j then val.satisfiesAt j φ else true)
+
+  def Valuation.isoToFinSetEquiv {frame : KripkeFrame n}: (Finset (KripkeGameVars × frame.Node)) ≃ frame.Valuation :=
+    finsetProdEquivCurriedCharacteristic
+
+  def allValuations (frame : KripkeFrame n) : Finset (frame.Valuation) :=
+    let valuationsAsPsets := (Finset.product KripkeGameVars.all frame.allNodes).powerset
+    valuationsAsPsets.map ((@KripkeFrame.Valuation.isoToFinSetEquiv _ frame).toEmbedding)
+
+  def Node.satisfiesForAllValuations {frame : KripkeFrame n} (i : frame.Node) (fml : ModalFormula) : Bool :=
+    decide (∀val ∈ frame.allValuations, val.satisfiesAt i fml)
+
+  def countSatisfyingNodes (frame : KripkeFrame n) (fml : ModalFormula) : ℕ :=
+    (frame.allNodes.filter (fun i => i.satisfiesForAllValuations fml)).card
+
+  lemma countSatisfyingNodes_leq_frameSize
+    (frame : KripkeFrame n) (fml : ModalFormula) : frame.countSatisfyingNodes fml ≤ n := by
+    simp only [KripkeFrame.countSatisfyingNodes]
+    simp only [← frame.allNodes_card_eq_frameSize]
+    apply Finset.card_filter_le
+end KripkeFrame
+
+structure KripkeGameVisibleState where
+  frameSize : ℕ
+  accessiblityRelationSize : Fin (frameSize * frameSize + 1)
+  queriesAndAnswers : List (ModalFormula × Fin (frameSize + 1))
+
+namespace KripkeGameVisibleState
+  def allPossibleInitialVisibleStates : Finset KripkeGameVisibleState :=
+    let frameSize := 4
+    let maxRelSize := frameSize * frameSize
+    let mapRelSizeToState := fun (n : Fin (maxRelSize + 1)) =>
+      {
+        frameSize := frameSize,
+        accessiblityRelationSize := n,
+        queriesAndAnswers := []
+        : KripkeGameVisibleState
+      }
+    let mappingInjective: Function.Injective mapRelSizeToState := by
+      intro n1 n2 h; simp only [mapRelSizeToState] at h; injection h
+    (Finset.univ : Finset (Fin (4 * 4 + 1))).map ⟨mapRelSizeToState, mappingInjective⟩
+
+  def withNewQueryAndAnswer (state : KripkeGameVisibleState) (query : ModalFormula) (answer : Fin (state.frameSize + 1)) : KripkeGameVisibleState :=
+    { state with queriesAndAnswers := (query, answer) :: state.queriesAndAnswers }
+
+  def possibleFramesUptoIso (state : KripkeGameVisibleState) : Finset (KripkeFrame state.frameSize) :=
+    sorry
+
+  def possibleFramesUptoIsoCard (state : KripkeGameVisibleState) : ℕ := state.possibleFramesUptoIso.card
+
+  inductive WinningStrategy : (n: ℕ) -> (state: KripkeGameVisibleState) -> Type where
+    | withExhaustiveSearch : possibleFramesUptoIsoCard state ≤ n -> WinningStrategy n state
+    | withParticularQuery : (nextQuery : ModalFormula) ->
+                  (Π answer : Fin (state.frameSize + 1), WinningStrategy n (state.withNewQueryAndAnswer nextQuery answer)) ->
+                  WinningStrategy (n + 1) state
+end KripkeGameVisibleState
+
+def kripkeGame_winning_strategy : ∀state ∈ KripkeGameVisibleState.allPossibleInitialVisibleStates,
+                                  KripkeGameVisibleState.WinningStrategy 10 state :=
+  sorry
