KripkeGameAnalysis/GenericExtras/FinsetEquivCharacteristic.lean
@@ -1,0 +1,13 @@
+import Mathlib.Data.Fintype.Basic
+import Mathlib.Data.Fintype.Prod
+
+def finsetEquivCharacteristic [Fintype α] [DecidableEq α] : Finset α ≃ (α → Bool) :=
+{ toFun := fun s a => decide (a ∈ s),
+  invFun := fun f => Finset.univ.filter (fun a => f a = true),
+  left_inv := by intro s; simp,
+  right_inv := by intro f; simp
+}
+
+def finsetProdEquivCurriedCharacteristic [Fintype α] [Fintype β] [DecidableEq α] [DecidableEq β]
+  : Finset (α × β) ≃ (α → β → Bool) :=
+  finsetEquivCharacteristic.trans (Equiv.curry _ _ _)
